testdata/cue/integer_keyword_expressions.cue
@@ -1,0 +1,5 @@
+divValue:   -7 div 3
+modValue:   -7 mod 3
+quoValue:   -7 quo 3
+remValue:   -7 rem 3
+precedence: 1 + 7 div 3
